compiler/src/compiler/FlatImp.v
@@ -393,11 +393,11 @@ Module exec.
             exists l', map.putmany_of_list_zip resvars resvals l = Some l' /\
             forall m', map.split m' mKeep mReceive ->
             post (((mGive, action, argvals), (mReceive, resvals)) :: t) m' l'
-                 (addMetricInstructions 1
-                 (addMetricStores 1
-                 (addMetricLoads 2 mc)))) ->
+                 (addMetricInstructions 100
+                 (addMetricJumps 100
+                 (addMetricStores 100
+                 (addMetricLoads 100 mc))))) ->
         exec (SInteract resvars action argvars) t m l mc post
-        (* TODO check SInteract case costs *)
     | call: forall t m l mc binds fname args params rets fbody argvs st0 post outcome,
         map.get e fname = Some (params, rets, fbody) ->
         map.getmany_of_list l args = Some argvs ->
